Updated to new, ocally installed metacoq (see install.txt), allowing use of qualified names in extraction. Alsu added missing file

theories/L/Tactics/GenEncode.v
@@ -6,14 +6,6 @@ Export String.StringSyntax.
 Import MonadNotation.
 Open Scope string_scope.
 
-(** *** Generation of encoding functions *)
-
-Fixpoint mkLApp (s : term) (L : list term) :=
-  match L with
-  | [] => s
-  | t :: L => mkLApp (tApp (tConstruct (mkInd "L.L.term" 0) 1 []) [s; t]) L
-  end.
-
 Definition encode_arguments (B : term) (a i : nat) A_j :=
       A <- tmUnquoteTyped Type A_j ;;
       name <- (tmEval cbv (name_of A_j ++ "_term") >>=  Core.tmFreshName)  ;;
@@ -32,7 +24,11 @@ Definition mkMatch (t1 t2 d : Ast.term) (cases : nat -> list term -> Core.Templa
                           l' <- monad_map_i (insert_params FUEL Params) (skipn params l) ;;
                           t <- cases i l' ;; ret (args, t)) L ;; 
   ret (tCase (ind, params) (tLambda nAnon t1 t2) d
-                                                body).
+             body).
+
+MetaCoq Quote Definition tLproc := L.proc.
+MetaCoq Quote Definition tLredLe := L.redLe.
+
 
 Definition tmMatchCorrect (A : Type) : Core.TemplateMonad Prop :=
   t <- (tmEval hnf A >>= tmQuote) ;; 
@@ -45,47 +41,50 @@ Definition tmMatchCorrect (A : Type) : Core.TemplateMonad Prop :=
               args <- tmEval cbv (|ctr_types|);; 
               C <- monad_map_i (encode_arguments t args) ctr_types ;; 
               ret (stack (map (tLambda (nAnon)) ctr_types)
-                               (((fun s => mkAppList s C) (tRel (args + 2 * (num - i) - 1)))))
+                               (((fun s => mkLAppList s C) (tRel (args + 2 * (num - i) - 1)))))
            ) ;;
    E' <- Core.tmInferInstance None (registered A);;
    E <- tmGetMyOption E' "failed" ;;        
    t' <- ret (@enc A E);;
    l <- tmQuote t';;
    encn <- ret (tApp l [tRel (2*num) ]) ;;
-   lhs <- ret (mkLApp encn ((fix f n := match n with 0 => [] | S n => tRel (2 * n + 1) :: f n end ) num)) ;;
-   ter <- ret (tProd nAnon t (it (fun s : term => tProd nAnon tTerm (tProd nAnon (tApp (tConst "L.L.proc" []) [tRel 0]) s)) num ((tApp (tConst "L.L.redLe" []) [mkNat num; lhs; mtch]))));;
+   lhs <- ret (mkLAppList encn ((fix f n := match n with 0 => [] | S n => tRel (2 * n + 1) :: f n end ) num)) ;;
+   ter <- ret (tProd nAnon t (it (fun s : term => tProd nAnon tTerm (tProd nAnon (tApp tLproc [tRel 0]) s)) num ((tApp tLredLe [mkNat num; lhs; mtch]))));;
    ter <- tmEval cbv ter ;;
-   tmUnquoteTyped Prop (fixNames ter).
+   tmUnquoteTyped Prop ter.
 
 Definition matchlem n A := (Core.tmBind (tmMatchCorrect A) (fun m => tmLemma n m ;; ret tt)).
 
-Definition tmGenEncode (n : ident) (A : Type) :=
+Definition tmGenEncode (n : ident) (A : Type) : TemplateMonad _:=
   e <- tmEncode n A;;
-  e <- tmUnquoteTyped (encodable A) (tConst n []);;
+  tmp' <- tmLocate1 n;;
+  tmp <- match tmp' with
+          ConstRef n' => tmReturn n'
+        | _ => tmFail "internal error in tmGenEncode"
+        end;;
+  e <- tmUnquoteTyped (encodable A) (tConst tmp Instance.empty);;
   p <- Core.tmLemma (n ++ "_proc") (forall x : A, proc (@enc_f A e x)) ;;
   n2 <- tmEval cbv ((n ++ "_inj"));;
   i <- Core.tmLemma n2  (injective (@enc_f _ e)) ;;
   n3 <- tmEval cbv ("registered_" ++ n) ;;
-  d <- Core.tmDefinition n3  (@mk_registered A e p i);;
-  tmExistingInstance n3;;
+  d <- tmInstanceRed n3 None (@mk_registered A e p i);;
   m <- tmMatchCorrect A;;
   n4 <- tmEval cbv (n ++ "_correct") ;;
   (Core.tmBind (tmMatchCorrect A) (fun m => tmLemma n4 m ;; ret tt)).
 
+(*
 Definition tmGenEncode' (n : ident) (A : Type) :=
   e <- tmEncode n A;;
-  e <- tmUnquoteTyped (encodable A) (tConst n []);;
   p <- Core.tmLemma (n ++ "_proc") (forall x : A, proc (@enc_f A e x)) ;;
   n2 <- tmEval cbv ((n ++ "_inj"));;
   i <- Core.tmLemma n2  (injective (@enc_f _ e)) ;;
   n3 <- tmEval cbv ("registered_" ++ n) ;;
-  d <- Core.tmDefinition n3  (@mk_registered A e p i);;
-  tmExistingInstance n3 ;;
-  m <- tmMatchCorrect A ;; ret tt.
+  d <- tmInstanceRed n3 None  (@mk_registered A e p i);;
+  m <- tmMatchCorrect A ;; ret tt. *)
 
 (* TODO : use other methode instead, e.g. with typeclasses, as default obligation tactic is very fragile *)
 Global Obligation Tactic := try fold (injective (enc_f)); match goal with
-                           | [ |- forall x : ?X, proc ?f ] => register_proc
+                           | [ |- forall x : ?X, proc ?f ] => try register_proc
                            | [ |- injective ?f ] => register_inj
                            | [ |- context [_ >(<= _) _] ] => extract match
-                           end || Tactics.program_simpl.
+                                                          end || Tactics.program_simpl.
