theories/L/Datatypes/LComparison.v
@@ -3,7 +3,7 @@ From Undecidability.L Require Import Tactics.GenEncode.
 
 (** *** Encoding for Comparisons *)
 
-Run TemplateProgram (tmGenEncode "comparison_enc" comparison).
+MetaCoq Run (tmGenEncode "comparison_enc" comparison).
 Hint Resolve comparison_enc_correct : Lrewrite.
 
 
